TA_Network/TP_NTA_Reduction_Utils.thy
@@ -1,0 +1,312 @@
+theory TP_NTA_Reduction_Utils
+  imports TP_NTA_Reduction_Model_Checking
+begin
+
+text \<open>Generic helper lemmas (pure-HOL + Munta-global), factored out of the reduction proofs.\<close>
+
+lemma fold_union:
+  "fold (\<union>) S T =  \<Union> (set S) \<union> T"
+  by (induction S arbitrary: T) auto
+
+lemma fold_union':
+  "fold (\<union>) S {} =  \<Union> (set S)"
+  apply (subst fold_union)
+  apply (subst Un_empty_right)
+  ..
+
+lemma set_nthI:
+  assumes "n < length xs"
+  shows "xs ! n \<in> set xs" using assms in_set_conv_nth by auto
+
+lemma sum_list_eq:
+  assumes "distinct xs" "distinct ys" "set xs = set ys" 
+  shows "sum_list ((map f xs)::nat list) = sum_list (map f ys)"
+proof -
+  have "mset xs = mset ys" using assms set_eq_iff_mset_eq_distinct by blast
+  hence "mset (map f xs) = mset (map f ys)" by simp
+  hence "fold (+) (map f xs) 0 = fold (+) (map f ys) 0"
+    apply -
+    apply (rule fold_permuted_eq[where P = "\<lambda>_. True"])
+       apply simp
+      apply simp
+     apply simp
+    by simp
+  moreover
+  have "foldr (+) (map f xs) 0 = fold (+) (map f xs) 0"
+    apply (subst foldr_fold)
+    by auto
+  moreover
+  have "foldr (+) (map f ys) 0 = fold (+) (map f ys) 0"
+    apply (subst foldr_fold)
+    by auto
+  ultimately
+  show ?thesis unfolding sum_list.eq_foldr by argo
+qed
+
+lemma foldr_assoc: "foldr (+) xs (n + 0::nat) = (foldr (+) xs 0) + n"
+  apply (induction xs)
+   apply simp
+  subgoal for x xs
+    by auto
+  done
+
+lemma dom_map_of_map:
+  "dom (map_of (map (\<lambda> (a, b). (f a, g b)) xs)) = f ` fst ` set xs"
+  unfolding dom_map_of_conv_image_fst by (auto 4 3)
+
+lemma map_of_NoneI:
+  "map_of xs x = None" if "x \<notin> fst ` set xs"
+  by (simp add: map_of_eq_None_iff that)
+
+lemma map_const_eq_conv_length_eq:
+  "map (\<lambda>x. n) xs = map (\<lambda>y. m) ys \<longleftrightarrow> length xs = length ys \<and> ((xs \<noteq> []) \<longrightarrow> n = m)"
+  apply (rule iffI)
+   apply (induction xs arbitrary: ys)
+    apply simp
+  subgoal for x xs ys
+    apply (induction ys)
+    by auto
+  apply (induction xs arbitrary: ys)
+   apply simp
+  subgoal for x xs ys
+    apply (induction ys)
+    by auto
+  done
+
+lemma is_upds_inc_vars: 
+  assumes "set xs \<subseteq> dom v"
+      and "distinct xs"
+      and "upds = (map (\<lambda>v. (v, binop plus_int (var v) (exp.const n))) xs)"
+      and "v' = v(xs [\<mapsto>] map (\<lambda>x. x + n) (map (the o v) xs))"
+  shows "is_upds v upds v'"
+  using assms(1,2)
+  unfolding assms(3,4)
+proof (induction xs arbitrary: v)
+  case Nil
+  then show ?case 
+    apply simp
+    by (rule is_upds.intros)
+next
+  case (Cons x xs v)
+  have 1: "is_upd v (x, binop plus_int (var x) (exp.const n)) (v(x \<mapsto> the (v x) + n))" (is "is_upd v ?upd ?v'")
+    unfolding is_upd_def
+     apply (intro exI conjI)
+       apply (rule HOL.refl)
+      apply (rule check_bexp_is_val.intros(14)[of _ _ "the (v x)"])
+      apply (rule check_bexp_is_val.intros)
+       using Cons(2) apply auto[1]
+        apply (rule check_bexp_is_val.intros)
+       by simp
+   from Cons(3)
+   have "\<forall>x' \<in> set xs. x \<noteq> x'" by auto
+   hence 2: "map (the o v) xs = map (the o ?v') xs"
+     unfolding comp_def using fun_upd_other by auto
+
+   have "is_upds ?v' (map (\<lambda>v. (v, binop plus_int (var v) (exp.const n))) xs) (?v'(xs [\<mapsto>] map (\<lambda>x. x + n) (map (the \<circ> ?v') xs)))"
+     apply (rule Cons.IH)
+     using Cons(2,3) by auto
+   hence 3: "is_upds ?v' (map (\<lambda>v. (v, binop plus_int (var v) (exp.const n))) xs) (?v'(xs [\<mapsto>] map (\<lambda>x. x + n) (map (the \<circ> v) xs)))"
+     apply (subst 2) by simp
+   show ?case 
+    apply (subst list.map)+
+    apply (subst map_upds_Cons)
+     apply (rule is_upds.intros(2)[OF 1])
+     using 3 unfolding comp_apply by simp
+qed
+
+lemma single_upd_bounded:
+  assumes "bounded M v"
+      and "M x = Some (l, u)"
+      and "l \<le> y"
+      and "y \<le> u"
+    shows "bounded M (v(x \<mapsto> y))"
+proof -
+  from assms[simplified bounded_def]
+  have dom_v_M: "dom v = dom M"
+    and bounds: "\<forall>x \<in> dom v. fst (the (M x)) \<le> the (v x) \<and> the (v x) \<le> snd (the (M x))"
+    by auto
+  
+  from assms(2) dom_v_M
+  have dom': "dom (v (x \<mapsto> y)) = dom v" by auto
+
+  have "fst (the (M a)) \<le> the ((v (x \<mapsto> y)) a) \<and> the ((v (x \<mapsto> y)) a) \<le> snd (the (M a))" if "a \<in> dom (v (x \<mapsto> y))" for a
+  proof (cases "a = x")
+    case True
+    then show ?thesis using assms(2,3,4) by simp
+  next
+    case False
+    hence 1: "the (v a) = the ((v (x \<mapsto> y)) a)" using that by simp
+    
+    have "a \<in> dom v" using dom' that by argo
+    from bounds[THEN bspec, OF this]
+    show ?thesis unfolding 1 by simp
+  qed
+  with dom' dom_v_M
+  show ?thesis unfolding bounded_def by simp
+qed
+
+find_theorems name: "map_upds"
+
+lemma upds_bounded:
+  assumes "bounded M v"
+      and "length xs = length ys"
+      and "\<forall>n < length xs. \<exists>l u. M (xs ! n) = Some (l, u) \<and> l \<le> (ys ! n) \<and> (ys ! n) \<le> u"   
+    shows "bounded M (v(xs [\<mapsto>] ys))"
+  using assms
+proof (induction xs arbitrary: ys v)
+  case Nil
+  then show ?case by simp
+next
+  case (Cons x xs)
+  then obtain y' ys' where
+    ys': "ys = y'#ys'"
+    "length (x # xs) = length (y' # ys')" apply (cases ys) by simp+
+  obtain l u where
+    "M x = Some (l, u)"
+    "l \<le> y'"
+    "y' \<le> u" using Cons(4)[simplified ys'(1)] by auto
+  with Cons(2)
+  have 1: "Simple_Network_Language.bounded M (v(x \<mapsto> y'))" by (auto intro: single_upd_bounded)
+  have 2: "\<forall>n<length xs. \<exists>l u. M (xs ! n) = Some (l, u) \<and> l \<le> ys' ! n \<and> ys' ! n \<le> u"
+  proof (intro allI impI)
+    fix n
+    assume a: "n < length xs"
+    hence 1: "Suc n < length (x # xs)" by simp
+    have "xs ! n = (x # xs) ! Suc n" by simp
+    moreover
+    have "ys' ! n = (y' # ys') ! Suc n" using ys' by simp
+    ultimately
+    show "\<exists>l u. M (xs ! n) = Some (l, u) \<and> l \<le> ys' ! n \<and> ys' ! n \<le> u" using Cons(4)[simplified ys'(1), THEN spec[of _ "Suc n"], THEN mp[OF _ 1]] by simp 
+  qed
+  with 1 ys'(2) Cons(4)
+  have "Simple_Network_Language.bounded M ((v(x \<mapsto> y'))(xs [\<mapsto>] ys'))"
+    apply -
+    apply (rule Cons.IH)
+      apply assumption
+    by simp+
+  thus ?case unfolding ys'(1) by simp
+qed
+
+lemma all_zip_replicate:
+  assumes "x \<in> set xs"
+  shows "\<forall>m. (x, m) \<in> set (zip xs (replicate (length xs) n)) \<longrightarrow> m = n"
+  using assms
+proof (induction xs arbitrary: n x)
+  case Nil
+  then show ?case by simp
+next
+  case (Cons a as)
+  have IH: "\<forall>m. (x, m) \<in> set (zip as (replicate (length as) n)) \<longrightarrow> m = n"
+    using Cons apply (cases "x \<in> set as")
+     apply simp using set_zip_leftD by metis
+  show ?case 
+    apply (subst length_Cons)
+    apply (subst replicate.simps)
+    apply (subst zip_Cons_Cons)
+    apply (rule allI)
+    subgoal for m
+      apply (cases "m = n")
+       apply simp
+      apply (subst list.set)
+      using IH by auto
+    done
+qed
+
+lemma map_of_determ:
+  assumes "\<forall>m. (x, m) \<in> set xs \<longrightarrow> m = n"
+          and "(x, n) \<in> set xs"
+        shows "map_of xs x = Some n"
+  using assms
+proof (induction xs)
+  case Nil
+  then show ?case by simp
+next
+  case (Cons a xs)
+  obtain c d where
+    a: "a = (c, d)" by fastforce
+  then show ?case 
+  proof (cases "a = (x,n)")
+    case True
+    then show ?thesis by simp
+  next
+    case False
+    then 
+    consider "x \<noteq> c" | "x = c \<and> n \<noteq> d" using a by blast
+    then show ?thesis 
+    proof cases
+      case 1
+      hence "map_of (a # xs) x = map_of xs x" using a map_of_Cons_code by auto
+      moreover
+      have i: "(x, n) \<in> set xs" using Cons (3) a 1 by auto
+      moreover
+      from Cons(2) i 1 False a
+      have "\<forall>m. (x, m) \<in> set xs \<longrightarrow> m = n" by force
+      ultimately
+      show ?thesis using Cons.IH by metis
+    next
+      case 2
+      then show ?thesis using a Cons by simp
+    qed
+  qed
+qed
+
+lemma map_upds_with_replicate:
+  assumes "x \<in> set xs"
+  shows "(v(xs [\<mapsto>] (replicate (length xs) n))) x = Some n"
+proof -
+  have "(x, n) \<in> set (zip xs (replicate (length xs) n))"
+    apply (subst set_zip)
+    using length_replicate assms
+    using nth_replicate
+    by (auto simp: set_conv_nth)
+  thus ?thesis
+    using assms 
+    unfolding map_upds_def 
+    apply (subst map_add_find_right)
+     apply (rule map_of_determ)
+    apply (subst set_rev)
+    using all_zip_replicate
+    by (fast, auto)
+qed
+
+
+lemma map_upds_with_map:
+  assumes "x \<in> set xs"
+      and "length xs = length ys"
+  shows "(v(xs [\<mapsto>] (map (\<lambda>x. n) ys))) x = Some n"
+proof -
+  have "\<forall>m. (x, m) \<in> set (zip xs (map (\<lambda>x. n) ys)) \<longrightarrow> m = n"
+    apply (subst set_zip)
+    by auto
+  moreover
+  have "(x, n) \<in> set (zip xs (map (\<lambda>x. n) ys))"
+    apply (subst set_zip)
+    using assms
+    by (auto simp: set_conv_nth set_zip)
+  ultimately
+  show ?thesis
+    using assms unfolding map_upds_def 
+    apply (subst map_add_find_right)
+    by (auto intro: map_of_determ)
+qed
+
+lemma distinct_map_upds:
+  assumes "x \<in> set xs"
+      and "distinct xs"
+    shows "(v(xs [\<mapsto>] (map f xs))) x = Some (f x)"
+  using assms 
+  unfolding map_upds_def
+  apply (subst map_add_find_right)
+   apply (subst zip_rev[symmetric])
+    apply simp
+   apply (rule map_of_is_SomeI[where y = "f x"])
+    apply simp
+   apply (subst zip_rev)
+    apply simp
+   apply (subst set_rev)
+   apply (subst in_set_zip)
+   apply (subst (asm) in_set_conv_nth)
+  by auto
+
+  
+end
